feat: extend 196 witness chain to iterate 69

ReverseAddNext.fst
@@ -7637,3 +7637,454 @@ let local_profile_witness_668656536414767878767414635656756 () : Lemma (
   reverse_add_159876958854887988978955775977805_to_668656536414767878767414635656756 ();
   no_overflow_outer_sum_6_to_9_implies_next_witness next25_source;
   ()
+
+let next26_source : numeral 10 = next25_target
+
+let next26_reversed : numeral 10 =
+  [6; 6; 8; 6; 5; 6; 5; 3; 6; 4; 1; 4; 7; 6; 7; 8; 7; 8; 7; 6; 7; 4; 1; 4; 6; 3; 5; 6; 5; 6; 7; 5; 6]
+
+let next26_target : numeral 10 =
+  [2; 2; 6; 3; 1; 3; 1; 7; 2; 9; 2; 8; 4; 3; 5; 7; 5; 7; 5; 3; 5; 9; 2; 8; 2; 7; 0; 3; 1; 3; 6; 2; 3; 1]
+
+let reverse_list_next26_source () : Lemma (rev next26_source == next26_reversed) =
+  assert (rev [6] == [6]);
+  rev_cons 6 [6];
+  rev_cons 8 [6; 6];
+  rev_cons 6 [8; 6; 6];
+  rev_cons 5 [6; 8; 6; 6];
+  rev_cons 6 [5; 6; 8; 6; 6];
+  rev_cons 5 [6; 5; 6; 8; 6; 6];
+  rev_cons 3 [5; 6; 5; 6; 8; 6; 6];
+  rev_cons 6 [3; 5; 6; 5; 6; 8; 6; 6];
+  rev_cons 4 [6; 3; 5; 6; 5; 6; 8; 6; 6];
+  rev_cons 1 [4; 6; 3; 5; 6; 5; 6; 8; 6; 6];
+  rev_cons 4 [1; 4; 6; 3; 5; 6; 5; 6; 8; 6; 6];
+  rev_cons 7 [4; 1; 4; 6; 3; 5; 6; 5; 6; 8; 6; 6];
+  rev_cons 6 [7; 4; 1; 4; 6; 3; 5; 6; 5; 6; 8; 6; 6];
+  rev_cons 7 [6; 7; 4; 1; 4; 6; 3; 5; 6; 5; 6; 8; 6; 6];
+  rev_cons 8 [7; 6; 7; 4; 1; 4; 6; 3; 5; 6; 5; 6; 8; 6; 6];
+  rev_cons 7 [8; 7; 6; 7; 4; 1; 4; 6; 3; 5; 6; 5; 6; 8; 6; 6];
+  rev_cons 8 [7; 8; 7; 6; 7; 4; 1; 4; 6; 3; 5; 6; 5; 6; 8; 6; 6];
+  rev_cons 7 [8; 7; 8; 7; 6; 7; 4; 1; 4; 6; 3; 5; 6; 5; 6; 8; 6; 6];
+  rev_cons 6 [7; 8; 7; 8; 7; 6; 7; 4; 1; 4; 6; 3; 5; 6; 5; 6; 8; 6; 6];
+  rev_cons 7 [6; 7; 8; 7; 8; 7; 6; 7; 4; 1; 4; 6; 3; 5; 6; 5; 6; 8; 6; 6];
+  rev_cons 4 [7; 6; 7; 8; 7; 8; 7; 6; 7; 4; 1; 4; 6; 3; 5; 6; 5; 6; 8; 6; 6];
+  rev_cons 1 [4; 7; 6; 7; 8; 7; 8; 7; 6; 7; 4; 1; 4; 6; 3; 5; 6; 5; 6; 8; 6; 6];
+  rev_cons 4 [1; 4; 7; 6; 7; 8; 7; 8; 7; 6; 7; 4; 1; 4; 6; 3; 5; 6; 5; 6; 8; 6; 6];
+  rev_cons 6 [4; 1; 4; 7; 6; 7; 8; 7; 8; 7; 6; 7; 4; 1; 4; 6; 3; 5; 6; 5; 6; 8; 6; 6];
+  rev_cons 3 [6; 4; 1; 4; 7; 6; 7; 8; 7; 8; 7; 6; 7; 4; 1; 4; 6; 3; 5; 6; 5; 6; 8; 6; 6];
+  rev_cons 5 [3; 6; 4; 1; 4; 7; 6; 7; 8; 7; 8; 7; 6; 7; 4; 1; 4; 6; 3; 5; 6; 5; 6; 8; 6; 6];
+  rev_cons 6 [5; 3; 6; 4; 1; 4; 7; 6; 7; 8; 7; 8; 7; 6; 7; 4; 1; 4; 6; 3; 5; 6; 5; 6; 8; 6; 6];
+  rev_cons 5 [6; 5; 3; 6; 4; 1; 4; 7; 6; 7; 8; 7; 8; 7; 6; 7; 4; 1; 4; 6; 3; 5; 6; 5; 6; 8; 6; 6];
+  rev_cons 6 [5; 6; 5; 3; 6; 4; 1; 4; 7; 6; 7; 8; 7; 8; 7; 6; 7; 4; 1; 4; 6; 3; 5; 6; 5; 6; 8; 6; 6];
+  rev_cons 7 [6; 5; 6; 5; 3; 6; 4; 1; 4; 7; 6; 7; 8; 7; 8; 7; 6; 7; 4; 1; 4; 6; 3; 5; 6; 5; 6; 8; 6; 6];
+  rev_cons 5 [7; 6; 5; 6; 5; 3; 6; 4; 1; 4; 7; 6; 7; 8; 7; 8; 7; 6; 7; 4; 1; 4; 6; 3; 5; 6; 5; 6; 8; 6; 6];
+  rev_cons 6 [5; 7; 6; 5; 6; 5; 3; 6; 4; 1; 4; 7; 6; 7; 8; 7; 8; 7; 6; 7; 4; 1; 4; 6; 3; 5; 6; 5; 6; 8; 6; 6];
+  ()
+
+let value_next26_reversed_tail_20 () : Lemma (
+    value #10 [6; 7; 8; 7; 8; 7; 6; 7; 4; 1; 4; 6; 3; 5; 6; 5; 6; 7; 5; 6] == 65765653641476787876) =
+  value_cons #10 6 [7; 8; 7; 8; 7; 6; 7; 4; 1; 4; 6; 3; 5; 6; 5; 6; 7; 5; 6];
+  value_cons #10 7 [8; 7; 8; 7; 6; 7; 4; 1; 4; 6; 3; 5; 6; 5; 6; 7; 5; 6];
+  value_cons #10 8 [7; 8; 7; 6; 7; 4; 1; 4; 6; 3; 5; 6; 5; 6; 7; 5; 6];
+  value_cons #10 7 [8; 7; 6; 7; 4; 1; 4; 6; 3; 5; 6; 5; 6; 7; 5; 6];
+  value_cons #10 8 [7; 6; 7; 4; 1; 4; 6; 3; 5; 6; 5; 6; 7; 5; 6];
+  value_cons #10 7 [6; 7; 4; 1; 4; 6; 3; 5; 6; 5; 6; 7; 5; 6];
+  value_cons #10 6 [7; 4; 1; 4; 6; 3; 5; 6; 5; 6; 7; 5; 6];
+  value_cons #10 7 [4; 1; 4; 6; 3; 5; 6; 5; 6; 7; 5; 6];
+  value_cons #10 4 [1; 4; 6; 3; 5; 6; 5; 6; 7; 5; 6];
+  value_cons #10 1 [4; 6; 3; 5; 6; 5; 6; 7; 5; 6];
+  value_cons #10 4 [6; 3; 5; 6; 5; 6; 7; 5; 6];
+  value_cons #10 6 [3; 5; 6; 5; 6; 7; 5; 6];
+  value_cons #10 3 [5; 6; 5; 6; 7; 5; 6];
+  value_cons #10 5 [6; 5; 6; 7; 5; 6];
+  value_cons #10 6 [5; 6; 7; 5; 6];
+  value_cons #10 5 [6; 7; 5; 6];
+  value_cons #10 6 [7; 5; 6];
+  value_cons #10 7 [5; 6];
+  value_cons #10 5 [6];
+  value_cons #10 6 [];
+  ()
+
+let value_next26_reversed () : Lemma (
+    value next26_reversed == 657656536414767878767414635656866) =
+  value_cons #10 6 [6; 8; 6; 5; 6; 5; 3; 6; 4; 1; 4; 7];
+  value_cons #10 6 [8; 6; 5; 6; 5; 3; 6; 4; 1; 4; 7];
+  value_cons #10 8 [6; 5; 6; 5; 3; 6; 4; 1; 4; 7];
+  value_cons #10 6 [5; 6; 5; 3; 6; 4; 1; 4; 7];
+  value_cons #10 5 [6; 5; 3; 6; 4; 1; 4; 7];
+  value_cons #10 6 [5; 3; 6; 4; 1; 4; 7];
+  value_cons #10 5 [3; 6; 4; 1; 4; 7];
+  value_cons #10 3 [6; 4; 1; 4; 7];
+  value_cons #10 6 [4; 1; 4; 7];
+  value_cons #10 4 [1; 4; 7];
+  value_cons #10 1 [4; 7];
+  value_cons #10 4 [7];
+  value_cons #10 7 [];
+  value_next26_reversed_tail_20 ();
+  ()
+
+let value_next26_target_tail_20 () : Lemma (
+    value #10 [5; 7; 5; 7; 5; 3; 5; 9; 2; 8; 2; 7; 0; 3; 1; 3; 6; 2; 3; 1] == 13263130728295357575) =
+  value_cons #10 5 [7; 5; 7; 5; 3; 5; 9; 2; 8; 2; 7; 0; 3; 1; 3; 6; 2; 3; 1];
+  value_cons #10 7 [5; 7; 5; 3; 5; 9; 2; 8; 2; 7; 0; 3; 1; 3; 6; 2; 3; 1];
+  value_cons #10 5 [7; 5; 3; 5; 9; 2; 8; 2; 7; 0; 3; 1; 3; 6; 2; 3; 1];
+  value_cons #10 7 [5; 3; 5; 9; 2; 8; 2; 7; 0; 3; 1; 3; 6; 2; 3; 1];
+  value_cons #10 5 [3; 5; 9; 2; 8; 2; 7; 0; 3; 1; 3; 6; 2; 3; 1];
+  value_cons #10 3 [5; 9; 2; 8; 2; 7; 0; 3; 1; 3; 6; 2; 3; 1];
+  value_cons #10 5 [9; 2; 8; 2; 7; 0; 3; 1; 3; 6; 2; 3; 1];
+  value_cons #10 9 [2; 8; 2; 7; 0; 3; 1; 3; 6; 2; 3; 1];
+  value_cons #10 2 [8; 2; 7; 0; 3; 1; 3; 6; 2; 3; 1];
+  value_cons #10 8 [2; 7; 0; 3; 1; 3; 6; 2; 3; 1];
+  value_cons #10 2 [7; 0; 3; 1; 3; 6; 2; 3; 1];
+  value_cons #10 7 [0; 3; 1; 3; 6; 2; 3; 1];
+  value_cons #10 0 [3; 1; 3; 6; 2; 3; 1];
+  value_cons #10 3 [1; 3; 6; 2; 3; 1];
+  value_cons #10 1 [3; 6; 2; 3; 1];
+  value_cons #10 3 [6; 2; 3; 1];
+  value_cons #10 6 [2; 3; 1];
+  value_cons #10 2 [3; 1];
+  value_cons #10 3 [1];
+  value_cons #10 1 [];
+  ()
+
+let value_next26_target () : Lemma (
+    value next26_target == 1326313072829535757534829271313622) =
+  value_cons #10 2 [2; 6; 3; 1; 3; 1; 7; 2; 9; 2; 8; 4; 3];
+  value_cons #10 2 [6; 3; 1; 3; 1; 7; 2; 9; 2; 8; 4; 3];
+  value_cons #10 6 [3; 1; 3; 1; 7; 2; 9; 2; 8; 4; 3];
+  value_cons #10 3 [1; 3; 1; 7; 2; 9; 2; 8; 4; 3];
+  value_cons #10 1 [3; 1; 7; 2; 9; 2; 8; 4; 3];
+  value_cons #10 3 [1; 7; 2; 9; 2; 8; 4; 3];
+  value_cons #10 1 [7; 2; 9; 2; 8; 4; 3];
+  value_cons #10 7 [2; 9; 2; 8; 4; 3];
+  value_cons #10 2 [9; 2; 8; 4; 3];
+  value_cons #10 9 [2; 8; 4; 3];
+  value_cons #10 2 [8; 4; 3];
+  value_cons #10 8 [4; 3];
+  value_cons #10 4 [3];
+  value_cons #10 3 [];
+  value_next26_target_tail_20 ();
+  ()
+
+let canonical_next26_reversed () : Lemma (canonical #10 next26_reversed) =
+  assert (canonical #10 [6]);
+  canonical_cons #10 5 [6];
+  canonical_cons #10 7 [5; 6];
+  canonical_cons #10 6 [7; 5; 6];
+  canonical_cons #10 5 [6; 7; 5; 6];
+  canonical_cons #10 6 [5; 6; 7; 5; 6];
+  canonical_cons #10 5 [6; 5; 6; 7; 5; 6];
+  canonical_cons #10 3 [5; 6; 5; 6; 7; 5; 6];
+  canonical_cons #10 6 [3; 5; 6; 5; 6; 7; 5; 6];
+  canonical_cons #10 4 [6; 3; 5; 6; 5; 6; 7; 5; 6];
+  canonical_cons #10 1 [4; 6; 3; 5; 6; 5; 6; 7; 5; 6];
+  canonical_cons #10 4 [1; 4; 6; 3; 5; 6; 5; 6; 7; 5; 6];
+  canonical_cons #10 7 [4; 1; 4; 6; 3; 5; 6; 5; 6; 7; 5; 6];
+  canonical_cons #10 6 [7; 4; 1; 4; 6; 3; 5; 6; 5; 6; 7; 5; 6];
+  canonical_cons #10 7 [6; 7; 4; 1; 4; 6; 3; 5; 6; 5; 6; 7; 5; 6];
+  canonical_cons #10 8 [7; 6; 7; 4; 1; 4; 6; 3; 5; 6; 5; 6; 7; 5; 6];
+  canonical_cons #10 7 [8; 7; 6; 7; 4; 1; 4; 6; 3; 5; 6; 5; 6; 7; 5; 6];
+  canonical_cons #10 8 [7; 8; 7; 6; 7; 4; 1; 4; 6; 3; 5; 6; 5; 6; 7; 5; 6];
+  canonical_cons #10 7 [8; 7; 8; 7; 6; 7; 4; 1; 4; 6; 3; 5; 6; 5; 6; 7; 5; 6];
+  canonical_cons #10 6 [7; 8; 7; 8; 7; 6; 7; 4; 1; 4; 6; 3; 5; 6; 5; 6; 7; 5; 6];
+  canonical_cons #10 7 [6; 7; 8; 7; 8; 7; 6; 7; 4; 1; 4; 6; 3; 5; 6; 5; 6; 7; 5; 6];
+  canonical_cons #10 4 [7; 6; 7; 8; 7; 8; 7; 6; 7; 4; 1; 4; 6; 3; 5; 6; 5; 6; 7; 5; 6];
+  canonical_cons #10 1 [4; 7; 6; 7; 8; 7; 8; 7; 6; 7; 4; 1; 4; 6; 3; 5; 6; 5; 6; 7; 5; 6];
+  canonical_cons #10 4 [1; 4; 7; 6; 7; 8; 7; 8; 7; 6; 7; 4; 1; 4; 6; 3; 5; 6; 5; 6; 7; 5; 6];
+  canonical_cons #10 6 [4; 1; 4; 7; 6; 7; 8; 7; 8; 7; 6; 7; 4; 1; 4; 6; 3; 5; 6; 5; 6; 7; 5; 6];
+  canonical_cons #10 3 [6; 4; 1; 4; 7; 6; 7; 8; 7; 8; 7; 6; 7; 4; 1; 4; 6; 3; 5; 6; 5; 6; 7; 5; 6];
+  canonical_cons #10 5 [3; 6; 4; 1; 4; 7; 6; 7; 8; 7; 8; 7; 6; 7; 4; 1; 4; 6; 3; 5; 6; 5; 6; 7; 5; 6];
+  canonical_cons #10 6 [5; 3; 6; 4; 1; 4; 7; 6; 7; 8; 7; 8; 7; 6; 7; 4; 1; 4; 6; 3; 5; 6; 5; 6; 7; 5; 6];
+  canonical_cons #10 5 [6; 5; 3; 6; 4; 1; 4; 7; 6; 7; 8; 7; 8; 7; 6; 7; 4; 1; 4; 6; 3; 5; 6; 5; 6; 7; 5; 6];
+  canonical_cons #10 6 [5; 6; 5; 3; 6; 4; 1; 4; 7; 6; 7; 8; 7; 8; 7; 6; 7; 4; 1; 4; 6; 3; 5; 6; 5; 6; 7; 5; 6];
+  canonical_cons #10 8 [6; 5; 6; 5; 3; 6; 4; 1; 4; 7; 6; 7; 8; 7; 8; 7; 6; 7; 4; 1; 4; 6; 3; 5; 6; 5; 6; 7; 5; 6];
+  canonical_cons #10 6 [8; 6; 5; 6; 5; 3; 6; 4; 1; 4; 7; 6; 7; 8; 7; 8; 7; 6; 7; 4; 1; 4; 6; 3; 5; 6; 5; 6; 7; 5; 6];
+  canonical_cons #10 6 [6; 8; 6; 5; 6; 5; 3; 6; 4; 1; 4; 7; 6; 7; 8; 7; 8; 7; 6; 7; 4; 1; 4; 6; 3; 5; 6; 5; 6; 7; 5; 6];
+  ()
+
+let canonical_next26_target () : Lemma (canonical #10 next26_target) =
+  assert (canonical #10 [1]);
+  canonical_cons #10 3 [1];
+  canonical_cons #10 2 [3; 1];
+  canonical_cons #10 6 [2; 3; 1];
+  canonical_cons #10 3 [6; 2; 3; 1];
+  canonical_cons #10 1 [3; 6; 2; 3; 1];
+  canonical_cons #10 3 [1; 3; 6; 2; 3; 1];
+  canonical_cons #10 0 [3; 1; 3; 6; 2; 3; 1];
+  canonical_cons #10 7 [0; 3; 1; 3; 6; 2; 3; 1];
+  canonical_cons #10 2 [7; 0; 3; 1; 3; 6; 2; 3; 1];
+  canonical_cons #10 8 [2; 7; 0; 3; 1; 3; 6; 2; 3; 1];
+  canonical_cons #10 2 [8; 2; 7; 0; 3; 1; 3; 6; 2; 3; 1];
+  canonical_cons #10 9 [2; 8; 2; 7; 0; 3; 1; 3; 6; 2; 3; 1];
+  canonical_cons #10 5 [9; 2; 8; 2; 7; 0; 3; 1; 3; 6; 2; 3; 1];
+  canonical_cons #10 3 [5; 9; 2; 8; 2; 7; 0; 3; 1; 3; 6; 2; 3; 1];
+  canonical_cons #10 5 [3; 5; 9; 2; 8; 2; 7; 0; 3; 1; 3; 6; 2; 3; 1];
+  canonical_cons #10 7 [5; 3; 5; 9; 2; 8; 2; 7; 0; 3; 1; 3; 6; 2; 3; 1];
+  canonical_cons #10 5 [7; 5; 3; 5; 9; 2; 8; 2; 7; 0; 3; 1; 3; 6; 2; 3; 1];
+  canonical_cons #10 7 [5; 7; 5; 3; 5; 9; 2; 8; 2; 7; 0; 3; 1; 3; 6; 2; 3; 1];
+  canonical_cons #10 5 [7; 5; 7; 5; 3; 5; 9; 2; 8; 2; 7; 0; 3; 1; 3; 6; 2; 3; 1];
+  canonical_cons #10 3 [5; 7; 5; 7; 5; 3; 5; 9; 2; 8; 2; 7; 0; 3; 1; 3; 6; 2; 3; 1];
+  canonical_cons #10 4 [3; 5; 7; 5; 7; 5; 3; 5; 9; 2; 8; 2; 7; 0; 3; 1; 3; 6; 2; 3; 1];
+  canonical_cons #10 8 [4; 3; 5; 7; 5; 7; 5; 3; 5; 9; 2; 8; 2; 7; 0; 3; 1; 3; 6; 2; 3; 1];
+  canonical_cons #10 2 [8; 4; 3; 5; 7; 5; 7; 5; 3; 5; 9; 2; 8; 2; 7; 0; 3; 1; 3; 6; 2; 3; 1];
+  canonical_cons #10 9 [2; 8; 4; 3; 5; 7; 5; 7; 5; 3; 5; 9; 2; 8; 2; 7; 0; 3; 1; 3; 6; 2; 3; 1];
+  canonical_cons #10 2 [9; 2; 8; 4; 3; 5; 7; 5; 7; 5; 3; 5; 9; 2; 8; 2; 7; 0; 3; 1; 3; 6; 2; 3; 1];
+  canonical_cons #10 7 [2; 9; 2; 8; 4; 3; 5; 7; 5; 7; 5; 3; 5; 9; 2; 8; 2; 7; 0; 3; 1; 3; 6; 2; 3; 1];
+  canonical_cons #10 1 [7; 2; 9; 2; 8; 4; 3; 5; 7; 5; 7; 5; 3; 5; 9; 2; 8; 2; 7; 0; 3; 1; 3; 6; 2; 3; 1];
+  canonical_cons #10 3 [1; 7; 2; 9; 2; 8; 4; 3; 5; 7; 5; 7; 5; 3; 5; 9; 2; 8; 2; 7; 0; 3; 1; 3; 6; 2; 3; 1];
+  canonical_cons #10 1 [3; 1; 7; 2; 9; 2; 8; 4; 3; 5; 7; 5; 7; 5; 3; 5; 9; 2; 8; 2; 7; 0; 3; 1; 3; 6; 2; 3; 1];
+  canonical_cons #10 3 [1; 3; 1; 7; 2; 9; 2; 8; 4; 3; 5; 7; 5; 7; 5; 3; 5; 9; 2; 8; 2; 7; 0; 3; 1; 3; 6; 2; 3; 1];
+  canonical_cons #10 6 [3; 1; 3; 1; 7; 2; 9; 2; 8; 4; 3; 5; 7; 5; 7; 5; 3; 5; 9; 2; 8; 2; 7; 0; 3; 1; 3; 6; 2; 3; 1];
+  canonical_cons #10 2 [6; 3; 1; 3; 1; 7; 2; 9; 2; 8; 4; 3; 5; 7; 5; 7; 5; 3; 5; 9; 2; 8; 2; 7; 0; 3; 1; 3; 6; 2; 3; 1];
+  canonical_cons #10 2 [2; 6; 3; 1; 3; 1; 7; 2; 9; 2; 8; 4; 3; 5; 7; 5; 7; 5; 3; 5; 9; 2; 8; 2; 7; 0; 3; 1; 3; 6; 2; 3; 1];
+  ()
+
+let reverse_digits_next26_source () : Lemma (
+    reverse_digits #10 next26_source == next26_reversed) =
+  ReverseAddNext.canonical_next25_target ();
+  reverse_list_next26_source ();
+  value_next26_reversed ();
+  canonical_next26_reversed ();
+  reverse_digits_canonical #10 next26_source;
+  normalize_value #10 (rev next26_source);
+  assert (value (reverse_digits #10 next26_source) ==
+    657656536414767878767414635656866);
+  digits_of_nat_of_canonical #10 (reverse_digits #10 next26_source);
+  digits_of_nat_of_canonical #10 next26_reversed;
+  assert (reverse_digits #10 next26_source == next26_reversed);
+  ()
+
+let reverse_add_668656536414767878767414635656756_to_1326313072829535757534829271313622 () : Lemma (
+    reverse_add #10 next26_source == next26_target) =
+  ReverseAddNext.canonical_next25_target ();
+  reverse_add_value #10 next26_source;
+  ReverseAddNext.value_next25_target ();
+  reverse_digits_next26_source ();
+  value_next26_reversed ();
+  value_next26_target ();
+  assert (value (reverse_add #10 next26_source) ==
+    1326313072829535757534829271313622);
+  reverse_add_canonical #10 next26_source;
+  digits_of_nat_of_canonical #10 (reverse_add #10 next26_source);
+  canonical_next26_target ();
+  digits_of_nat_of_canonical #10 next26_target;
+  assert (reverse_add #10 next26_source == next26_target);
+  ()
+
+let trace_digits_profile_668656536414767878767414635656756 () : Lemma (
+    trace_digits next26_source == next26_target) =
+  reverse_add_668656536414767878767414635656756_to_1326313072829535757534829271313622 ();
+  trace_digits_equals_reverse_add next26_source;
+  assert (trace_digits next26_source == next26_target);
+  ()
+
+let trace_carries_next26_source () : Lemma (trace_carries next26_source ==
+    [0; 1; 1; 1; 1; 1; 1; 1; 0; 1; 0; 0; 0; 1; 1; 1; 1; 1; 1; 1; 1; 1; 0; 0; 0; 1; 0; 1; 1; 1; 1; 1; 1; 1]) =
+  reverse_list_next26_source ();
+  assert (trace_carries next26_source ==
+    (add_trace #10 next26_source next26_reversed 0).carries);
+  add_trace_carries_step #10 6 6
+    [5; 7; 6; 5; 6; 5; 3; 6; 4; 1; 4; 7; 6; 7; 8; 7; 8; 7; 6; 7; 4; 1; 4; 6; 3; 5; 6; 5; 6; 8; 6; 6]
+    [6; 8; 6; 5; 6; 5; 3; 6; 4; 1; 4; 7; 6; 7; 8; 7; 8; 7; 6; 7; 4; 1; 4; 6; 3; 5; 6; 5; 6; 7; 5; 6] 0;
+  add_trace_carries_step #10 5 6
+    [7; 6; 5; 6; 5; 3; 6; 4; 1; 4; 7; 6; 7; 8; 7; 8; 7; 6; 7; 4; 1; 4; 6; 3; 5; 6; 5; 6; 8; 6; 6]
+    [8; 6; 5; 6; 5; 3; 6; 4; 1; 4; 7; 6; 7; 8; 7; 8; 7; 6; 7; 4; 1; 4; 6; 3; 5; 6; 5; 6; 7; 5; 6] 1;
+  add_trace_carries_step #10 7 8
+    [6; 5; 6; 5; 3; 6; 4; 1; 4; 7; 6; 7; 8; 7; 8; 7; 6; 7; 4; 1; 4; 6; 3; 5; 6; 5; 6; 8; 6; 6]
+    [6; 5; 6; 5; 3; 6; 4; 1; 4; 7; 6; 7; 8; 7; 8; 7; 6; 7; 4; 1; 4; 6; 3; 5; 6; 5; 6; 7; 5; 6] 1;
+  add_trace_carries_step #10 6 6
+    [5; 6; 5; 3; 6; 4; 1; 4; 7; 6; 7; 8; 7; 8; 7; 6; 7; 4; 1; 4; 6; 3; 5; 6; 5; 6; 8; 6; 6]
+    [5; 6; 5; 3; 6; 4; 1; 4; 7; 6; 7; 8; 7; 8; 7; 6; 7; 4; 1; 4; 6; 3; 5; 6; 5; 6; 7; 5; 6] 1;
+  add_trace_carries_step #10 5 5
+    [6; 5; 3; 6; 4; 1; 4; 7; 6; 7; 8; 7; 8; 7; 6; 7; 4; 1; 4; 6; 3; 5; 6; 5; 6; 8; 6; 6]
+    [6; 5; 3; 6; 4; 1; 4; 7; 6; 7; 8; 7; 8; 7; 6; 7; 4; 1; 4; 6; 3; 5; 6; 5; 6; 7; 5; 6] 1;
+  add_trace_carries_step #10 6 6
+    [5; 3; 6; 4; 1; 4; 7; 6; 7; 8; 7; 8; 7; 6; 7; 4; 1; 4; 6; 3; 5; 6; 5; 6; 8; 6; 6]
+    [5; 3; 6; 4; 1; 4; 7; 6; 7; 8; 7; 8; 7; 6; 7; 4; 1; 4; 6; 3; 5; 6; 5; 6; 7; 5; 6] 1;
+  add_trace_carries_step #10 5 5
+    [3; 6; 4; 1; 4; 7; 6; 7; 8; 7; 8; 7; 6; 7; 4; 1; 4; 6; 3; 5; 6; 5; 6; 8; 6; 6]
+    [3; 6; 4; 1; 4; 7; 6; 7; 8; 7; 8; 7; 6; 7; 4; 1; 4; 6; 3; 5; 6; 5; 6; 7; 5; 6] 1;
+  add_trace_carries_step #10 3 3
+    [6; 4; 1; 4; 7; 6; 7; 8; 7; 8; 7; 6; 7; 4; 1; 4; 6; 3; 5; 6; 5; 6; 8; 6; 6]
+    [6; 4; 1; 4; 7; 6; 7; 8; 7; 8; 7; 6; 7; 4; 1; 4; 6; 3; 5; 6; 5; 6; 7; 5; 6] 1;
+  add_trace_carries_step #10 6 6
+    [4; 1; 4; 7; 6; 7; 8; 7; 8; 7; 6; 7; 4; 1; 4; 6; 3; 5; 6; 5; 6; 8; 6; 6]
+    [4; 1; 4; 7; 6; 7; 8; 7; 8; 7; 6; 7; 4; 1; 4; 6; 3; 5; 6; 5; 6; 7; 5; 6] 0;
+  add_trace_carries_step #10 4 4
+    [1; 4; 7; 6; 7; 8; 7; 8; 7; 6; 7; 4; 1; 4; 6; 3; 5; 6; 5; 6; 8; 6; 6]
+    [1; 4; 7; 6; 7; 8; 7; 8; 7; 6; 7; 4; 1; 4; 6; 3; 5; 6; 5; 6; 7; 5; 6] 1;
+  add_trace_carries_step #10 1 1
+    [4; 7; 6; 7; 8; 7; 8; 7; 6; 7; 4; 1; 4; 6; 3; 5; 6; 5; 6; 8; 6; 6]
+    [4; 7; 6; 7; 8; 7; 8; 7; 6; 7; 4; 1; 4; 6; 3; 5; 6; 5; 6; 7; 5; 6] 0;
+  add_trace_carries_step #10 4 4
+    [7; 6; 7; 8; 7; 8; 7; 6; 7; 4; 1; 4; 6; 3; 5; 6; 5; 6; 8; 6; 6]
+    [7; 6; 7; 8; 7; 8; 7; 6; 7; 4; 1; 4; 6; 3; 5; 6; 5; 6; 7; 5; 6] 0;
+  add_trace_carries_step #10 7 7
+    [6; 7; 8; 7; 8; 7; 6; 7; 4; 1; 4; 6; 3; 5; 6; 5; 6; 8; 6; 6]
+    [6; 7; 8; 7; 8; 7; 6; 7; 4; 1; 4; 6; 3; 5; 6; 5; 6; 7; 5; 6] 0;
+  add_trace_carries_step #10 6 6
+    [7; 8; 7; 8; 7; 6; 7; 4; 1; 4; 6; 3; 5; 6; 5; 6; 8; 6; 6]
+    [7; 8; 7; 8; 7; 6; 7; 4; 1; 4; 6; 3; 5; 6; 5; 6; 7; 5; 6] 1;
+  add_trace_carries_step #10 7 7
+    [8; 7; 8; 7; 6; 7; 4; 1; 4; 6; 3; 5; 6; 5; 6; 8; 6; 6]
+    [8; 7; 8; 7; 6; 7; 4; 1; 4; 6; 3; 5; 6; 5; 6; 7; 5; 6] 1;
+  add_trace_carries_step #10 8 8
+    [7; 8; 7; 6; 7; 4; 1; 4; 6; 3; 5; 6; 5; 6; 8; 6; 6]
+    [7; 8; 7; 6; 7; 4; 1; 4; 6; 3; 5; 6; 5; 6; 7; 5; 6] 1;
+  add_trace_carries_step #10 7 7
+    [8; 7; 6; 7; 4; 1; 4; 6; 3; 5; 6; 5; 6; 8; 6; 6]
+    [8; 7; 6; 7; 4; 1; 4; 6; 3; 5; 6; 5; 6; 7; 5; 6] 1;
+  add_trace_carries_step #10 8 8
+    [7; 6; 7; 4; 1; 4; 6; 3; 5; 6; 5; 6; 8; 6; 6]
+    [7; 6; 7; 4; 1; 4; 6; 3; 5; 6; 5; 6; 7; 5; 6] 1;
+  add_trace_carries_step #10 7 7
+    [6; 7; 4; 1; 4; 6; 3; 5; 6; 5; 6; 8; 6; 6]
+    [6; 7; 4; 1; 4; 6; 3; 5; 6; 5; 6; 7; 5; 6] 1;
+  add_trace_carries_step #10 6 6
+    [7; 4; 1; 4; 6; 3; 5; 6; 5; 6; 8; 6; 6]
+    [7; 4; 1; 4; 6; 3; 5; 6; 5; 6; 7; 5; 6] 1;
+  add_trace_carries_step #10 7 7
+    [4; 1; 4; 6; 3; 5; 6; 5; 6; 8; 6; 6]
+    [4; 1; 4; 6; 3; 5; 6; 5; 6; 7; 5; 6] 1;
+  add_trace_carries_step #10 4 4
+    [1; 4; 6; 3; 5; 6; 5; 6; 8; 6; 6]
+    [1; 4; 6; 3; 5; 6; 5; 6; 7; 5; 6] 1;
+  add_trace_carries_step #10 1 1
+    [4; 6; 3; 5; 6; 5; 6; 8; 6; 6]
+    [4; 6; 3; 5; 6; 5; 6; 7; 5; 6] 0;
+  add_trace_carries_step #10 4 4
+    [6; 3; 5; 6; 5; 6; 8; 6; 6]
+    [6; 3; 5; 6; 5; 6; 7; 5; 6] 0;
+  add_trace_carries_step #10 6 6
+    [3; 5; 6; 5; 6; 8; 6; 6]
+    [3; 5; 6; 5; 6; 7; 5; 6] 0;
+  add_trace_carries_step #10 3 3
+    [5; 6; 5; 6; 8; 6; 6]
+    [5; 6; 5; 6; 7; 5; 6] 1;
+  add_trace_carries_step #10 5 5
+    [6; 5; 6; 8; 6; 6]
+    [6; 5; 6; 7; 5; 6] 0;
+  add_trace_carries_step #10 6 6
+    [5; 6; 8; 6; 6]
+    [5; 6; 7; 5; 6] 1;
+  add_trace_carries_step #10 5 5
+    [6; 8; 6; 6]
+    [6; 7; 5; 6] 1;
+  add_trace_carries_step #10 6 6
+    [8; 6; 6]
+    [7; 5; 6] 1;
+  add_trace_carries_step #10 8 7
+    [6; 6]
+    [5; 6] 1;
+  add_trace_carries_step #10 6 5
+    [6]
+    [6] 1;
+  add_trace_carries_step #10 6 6
+    []
+    [] 1;
+  assert ((add_trace #10 [] [] 1).carries == [1]);
+  assert ((add_trace #10 next26_source next26_reversed 0).carries == [0; 1; 1; 1; 1; 1; 1; 1; 0; 1; 0; 0; 0; 1; 1; 1; 1; 1; 1; 1; 1; 1; 0; 0; 0; 1; 0; 1; 1; 1; 1; 1; 1; 1]);
+  ()
+
+let trace_profile_shape_668656536414767878767414635656756 () : Lemma (
+    length (trace_digits next26_source) == length next26_source + 1) =
+  trace_digits_profile_668656536414767878767414635656756 ();
+  length_of_eq #(digit 10) (trace_digits next26_source) next26_target;
+  assert (length next26_target == length next26_source + 1);
+  ()
+
+let trace_profile_final_carry_668656536414767878767414635656756 () : Lemma (
+    nth (trace_carries next26_source) (length next26_source) == Some 1) =
+  trace_profile_shape_668656536414767878767414635656756 ();
+  ReverseAddContinuation.final_carry_from_overflow_length next26_source;
+  ()
+
+let trace_profile_sums_668656536414767878767414635656756 () : Lemma (
+    trace_sum_at next26_source 0 == 12 /\
+    trace_sum_at next26_source 9 == 8 /\
+    trace_sum_at next26_source 24 == 12) =
+  reverse_list_next26_source ();
+  ()
+
+let trace_profile_carry_facts_668656536414767878767414635656756 () : Lemma (
+    trace_carry_at next26_source 1 == 1 /\
+    trace_carry_at next26_source 32 == 1 /\
+    trace_carry_at next26_source 9 == 1 /\
+    trace_carry_at next26_source 33 == 1 /\
+    trace_carry_at next26_source 10 == 0 /\
+    trace_carry_at next26_source 24 == 0) =
+  trace_carries_next26_source ();
+  assert (trace_carry_at next26_source 1 == 1);
+  assert (trace_carry_at next26_source 32 == 1);
+  assert (trace_carry_at next26_source 9 == 1);
+  assert (trace_carry_at next26_source 33 == 1);
+  assert (trace_carry_at next26_source 10 == 0);
+  assert (trace_carry_at next26_source 24 == 0);
+  assert (trace_carries next26_source == [0; 1; 1; 1; 1; 1; 1; 1; 0; 1; 0; 0; 0; 1; 1; 1; 1; 1; 1; 1; 1; 1; 0; 0; 0; 1; 0; 1; 1; 1; 1; 1; 1; 1]);
+  ()
+
+let overflow_precondition_668656536414767878767414635656756 () : Lemma (
+    canonical #10 next26_source /\
+    next26_source <> [] /\
+    length (trace_digits next26_source) == length next26_source + 1 /\
+    nth (trace_carries next26_source) (length next26_source) == Some 1 /\
+    1 <= trace_sum_at next26_source 0 /\
+    trace_sum_at next26_source 0 <= 18 /\
+    trace_sum_at next26_source 0 <> 10 /\
+    exists (i:nat). 0 < i /\ i < length next26_source /\
+      trace_sum_at next26_source i +
+          trace_sum_at next26_source (length next26_source - i) +
+          trace_carry_at next26_source i +
+          trace_carry_at next26_source (length next26_source - i) >=
+        10 + 10 *
+          (trace_carry_at next26_source (i + 1) +
+           trace_carry_at next26_source (length next26_source - i + 1))) =
+  ReverseAddNext.canonical_next25_target ();
+  assert (next26_source <> []);
+  trace_profile_shape_668656536414767878767414635656756 ();
+  trace_profile_final_carry_668656536414767878767414635656756 ();
+  trace_profile_sums_668656536414767878767414635656756 ();
+  trace_profile_carry_facts_668656536414767878767414635656756 ();
+  assert (length (trace_digits next26_source) == length next26_source + 1);
+  assert (nth (trace_carries next26_source)
+    (length next26_source) == Some 1);
+  assert (trace_sum_at next26_source 0 == 12);
+  assert (trace_sum_at next26_source 9 == 8);
+  assert (trace_sum_at next26_source 24 == 12);
+  assert (trace_carry_at next26_source 1 == 1);
+  assert (trace_carry_at next26_source 32 == 1);
+  assert (trace_carry_at next26_source 9 == 1);
+  assert (trace_carry_at next26_source 33 == 1);
+  assert (trace_carry_at next26_source 10 == 0);
+  assert (trace_carry_at next26_source 24 == 0);
+  assert (1 <= trace_sum_at next26_source 0 /\
+    trace_sum_at next26_source 0 <= 18);
+  assert (trace_sum_at next26_source 0 <> 10);
+  let n : nat = length next26_source in
+  assert (0 < 9 /\ 9 < n);
+  assert (trace_sum_at next26_source 9 +
+      trace_sum_at next26_source (n - 9) +
+      trace_carry_at next26_source 9 +
+      trace_carry_at next26_source (n - 9) >=
+    10 + 10 *
+      (trace_carry_at next26_source (9 + 1) +
+       trace_carry_at next26_source (n - 9 + 1)));
+  exists_intro
+    (fun (i:nat) -> 0 < i /\ i < n /\
+      trace_sum_at next26_source i +
+          trace_sum_at next26_source (n - i) +
+          trace_carry_at next26_source i +
+          trace_carry_at next26_source (n - i) >=
+        10 + 10 *
+          (trace_carry_at next26_source (i + 1) +
+           trace_carry_at next26_source (n - i + 1)))
+    9;
+  ()
+
+let local_profile_witness_1326313072829535757534829271313622 () : Lemma (
+    trace_local_profile_complement_witness next26_target) =
+  overflow_precondition_668656536414767878767414635656756 ();
+  reverse_add_668656536414767878767414635656756_to_1326313072829535757534829271313622 ();
+  overflow_internal_cell_implies_next_witness next26_source;
+  ()
